Just in case

DeBruijnSSA/BinSyntax/Rewrite/Region/Compose/Product.lean
@@ -1,5 +1,6 @@
 import DeBruijnSSA.BinSyntax.Rewrite.Region.LSubst
 import DeBruijnSSA.BinSyntax.Rewrite.Region.Compose.Seq
+import DeBruijnSSA.BinSyntax.Rewrite.Term.Compose.Product
 import DeBruijnSSA.BinSyntax.Typing.Region.Compose
 
 namespace BinSyntax
@@ -19,17 +20,30 @@ def Eqv.rtimes {tyIn tyOut : Ty α} {Γ : Ctx α ε} {L : LCtx α}
 
 infixl:70 " ⋊ "  => Eqv.rtimes
 
+theorem Eqv.rtimes_eq_ret {tyIn tyOut : Ty α} {Γ : Ctx α ε} {L : LCtx α}
+  {tyLeft : Ty α} {r : Term.Eqv φ (⟨tyIn, ⊥⟩::Γ) ⟨tyOut, ⊥⟩}
+  : tyLeft ⋊ ret r = Eqv.ret (targets := L) (r.rtimes tyLeft) := by
+  simp only [Eqv.rtimes, vwk1_ret, ret_ret, let2_ret, Term.Eqv.rtimes_def']
+  rfl
+
 theorem Eqv.Pure.rtimes {tyIn tyOut : Ty α} {Γ : Ctx α ε} {L : LCtx α}
   (tyLeft : Ty α) {r : Eqv φ (⟨tyIn, ⊥⟩::Γ) (tyOut::L)}
-  : Eqv.Pure r → Eqv.Pure (tyLeft ⋊ r) := sorry
+  (hp : Eqv.Pure r) : Eqv.Pure (tyLeft ⋊ r) := let ⟨_, hp⟩ := hp; ⟨_, hp ▸ rtimes_eq_ret⟩
 
 def Eqv.braid {left right : Ty α} {Γ : Ctx α ε} {L : LCtx α}
   : Eqv φ (⟨left.prod right, ⊥⟩::Γ) ((right.prod left)::L)
   := Eqv.let2 (var 0 Ctx.Var.shead) $
   ret (pair (var 0 (by simp)) (var 1 (by simp)))
 
+theorem Eqv.braid_eq_ret {left right : Ty α} {Γ : Ctx α ε} {L : LCtx α}
+  : Eqv.braid (φ := φ) (left := left) (right := right) (Γ := Γ) (L := L) = Eqv.ret Term.Eqv.braid
+  := by
+  simp only [Eqv.braid, let2_ret]
+  rfl
+
 theorem Eqv.Pure.braid {left right : Ty α} {Γ : Ctx α ε} {L : LCtx α}
-  : Eqv.Pure (Eqv.braid (φ := φ) (left := left) (right := right) (Γ := Γ) (L := L)) := sorry
+  : Eqv.Pure (Eqv.braid (φ := φ) (left := left) (right := right) (Γ := Γ) (L := L))
+  := ⟨_, braid_eq_ret⟩
 
 theorem Eqv.repack {left right : Ty α} {rest : Ctx α ε} {targets : LCtx α}
   : Eqv.let2 (var 0 ⟨by simp, le_refl _⟩)
@@ -41,22 +55,16 @@ theorem Eqv.repack {left right : Ty α} {rest : Ctx α ε} {targets : LCtx α}
 theorem Eqv.braid_braid {left right : Ty α}
   : Eqv.braid ;; Eqv.braid
   = (Eqv.nil (φ := φ) (ty := left.prod right) (rest := rest) (targets := targets)) := by
-  stop
-  simp only [
-    braid, let2_seq, vwk1, vwk_let2, wk_var, wk_pair, Nat.liftWk, vwk_ret, Ctx.InS.liftn₂,
-    Nat.liftnWk, Nat.one_lt_ofNat, Nat.ofNat_pos, ↓reduceIte, ret_seq, vsubst_let2,
-    subst_pair, subst_var, Term.Subst.InS.get_0_subst0, let2_pair, let1_beta, vsubst_vsubst
-  ]
-  apply Eqv.repack
+  simp only [braid_eq_ret, ret_ret, Term.Eqv.braid_braid, ret_nil]
 
 theorem Eqv.rtimes_nil {ty : Ty α} {Γ : Ctx α ε} {L : LCtx α}
   (tyLeft : Ty α)
   : tyLeft ⋊ Eqv.nil = (Eqv.nil (φ := φ) (ty := tyLeft.prod ty) (rest := Γ) (targets := L)) := by
   simp only [rtimes, nil_vwk1, nil_seq, repack]
 
-theorem Eqv.rtimes_seq {A B C : Ty α} {Γ : Ctx α ε} {L : LCtx α}
+theorem Eqv.rtimes_rtimes {A B C : Ty α} {Γ : Ctx α ε} {L : LCtx α}
   (tyLeft : Ty α) (r : Eqv φ (⟨A, ⊥⟩::Γ) (B::L)) (s : Eqv φ (⟨B, ⊥⟩::Γ) (C::L))
-  : tyLeft ⋊ (r ;; s) = (tyLeft ⋊ r) ;; (tyLeft ⋊ s) := by
+  : (tyLeft ⋊ r) ;; (tyLeft ⋊ s) = tyLeft ⋊ (r ;; s) := by
   stop
   apply Eq.symm
   rw [rtimes, rtimes, let2_seq, seq_assoc, ret_seq]
@@ -71,12 +79,23 @@ theorem Eqv.rtimes_seq {A B C : Ty α} {Γ : Ctx α ε} {L : LCtx α}
   . simp [vwk1, vwk_vwk]
   . sorry
 
+theorem Eqv.vwk_lift_rtimes {A B : Ty α} {Γ Δ : Ctx α ε} {L : LCtx α}
+  {r : Eqv φ (⟨A, ⊥⟩::Δ) (B::L)} {ρ : Γ.InS Δ}
+  : (X ⋊ r).vwk (ρ.lift (le_refl _)) = X ⋊ (r.vwk (ρ.lift (le_refl _))) := by
+  simp [rtimes, vwk_lift_seq]
+  sorry
+
 def Eqv.ltimes {tyIn tyOut : Ty α} {Γ : Ctx α ε} {L : LCtx α}
   (r : Eqv φ (⟨tyIn, ⊥⟩::Γ) (tyOut::L)) (tyRight : Ty α)
   : Eqv φ (⟨tyIn.prod tyRight, ⊥⟩::Γ) ((tyOut.prod tyRight)::L)
   := Eqv.braid ;; tyRight ⋊ r ;; Eqv.braid
 
 infixl:70 " ⋉ "  => Eqv.ltimes
+
+theorem Eqv.ltimes_eq_ret {tyIn tyOut : Ty α} {Γ : Ctx α ε} {L : LCtx α}
+  {tyRight : Ty α} {r : Term.Eqv φ (⟨tyIn, ⊥⟩::Γ) ⟨tyOut, ⊥⟩}
+  : ret (targets := L) r ⋉ tyRight = ret (r.ltimes tyRight) := by
+  simp only [ltimes, braid_eq_ret, rtimes_eq_ret, ret_ret, Term.Eqv.braid_rtimes_braid]
 
 theorem Eqv.Pure.ltimes {tyIn tyOut : Ty α} {Γ : Ctx α ε} {L : LCtx α}
   {r : Eqv φ (⟨tyIn, ⊥⟩::Γ) (tyOut::L)} (hr : r.Pure) (tyRight : Ty α)
@@ -107,85 +126,118 @@ theorem Eqv.ltimes_nil {ty : Ty α} {Γ : Ctx α ε} {L : LCtx α}
   : Eqv.nil ⋉ tyRight = (Eqv.nil (φ := φ) (ty := ty.prod tyRight) (rest := Γ) (targets := L))
   := by rw [<-braid_rtimes_braid, rtimes_nil, seq_nil, braid_braid]
 
-theorem Eqv.ltimes_seq {A B C : Ty α} {Γ : Ctx α ε} {L : LCtx α}
+theorem Eqv.ltimes_ltimes {A B C : Ty α} {Γ : Ctx α ε} {L : LCtx α}
   (r : Eqv φ (⟨A, ⊥⟩::Γ) (B::L)) (s : Eqv φ (⟨B, ⊥⟩::Γ) (C::L))
-  : (r ;; s) ⋉ tyRight = (r ⋉ tyRight) ;; (s ⋉ tyRight) := by
-  simp only [<-braid_rtimes_braid, rtimes_seq, seq_assoc]
+  : (r ⋉ tyRight) ;; (s ⋉ tyRight) = (r ;; s) ⋉ tyRight := by
+  simp only [<-braid_rtimes_braid, <-rtimes_rtimes, seq_assoc]
   rw [<-seq_assoc braid braid, braid_braid, nil_seq]
 
-def Eqv.runit {ty : Ty α} {Γ : Ctx α ε} {L : LCtx α}
-  : Eqv φ (⟨ty.prod Ty.unit, ⊥⟩::Γ) (ty::L)
+def Eqv.pi_l {A B : Ty α} {Γ : Ctx α ε} {L : LCtx α}
+  : Eqv φ (⟨A.prod B, ⊥⟩::Γ) (A::L)
   := let2 (var 0 Ctx.Var.shead) (ret $ var 1 (by simp))
 
-def Eqv.runit_inv {ty : Ty α} {Γ : Ctx α ε} {L : LCtx α}
+def Eqv.runit {ty : Ty α} {Γ : Ctx α ε} {L : LCtx α}
   : Eqv φ (⟨ty, ⊥⟩::Γ) (ty.prod Ty.unit::L)
   := ret $ (pair (var 0 Ctx.Var.shead) (unit _))
 
+theorem Eqv.pi_l_eq_ret {Γ : Ctx α ε} {L : LCtx α}
+  : Eqv.pi_l (φ := φ) (A := A) (B := B) (Γ := Γ) (L := L) = Eqv.ret Term.Eqv.pi_l := by
+  simp only [Eqv.pi_l, let2_ret]
+  rfl
+
+theorem Eqv.runit_eq_ret {ty : Ty α} {Γ : Ctx α ε} {L : LCtx α}
+  : Eqv.runit (φ := φ) (ty := ty) (Γ := Γ) (L := L) = Eqv.ret Term.Eqv.runit := by
+  simp only [Eqv.runit, ret_ret]
+  rfl
+
+@[simp]
+theorem Eqv.vwk1_pi_l {Γ : Ctx α ε} {L : LCtx α}
+  : (pi_l (φ := φ) (A := A) (B := B) (Γ := Γ) (L := L)).vwk1 (inserted := inserted) = pi_l := rfl
+
+theorem Eqv.Pure.pi_l {Γ : Ctx α ε} {L : LCtx α}
+  : (pi_l (φ := φ) (A := A) (B := B) (Γ := Γ) (L := L)).Pure := ⟨_, pi_l_eq_ret⟩
+
 theorem Eqv.Pure.runit {ty : Ty α} {Γ : Ctx α ε} {L : LCtx α}
-  : (runit (φ := φ) (ty := ty) (Γ := Γ) (L := L)).Pure := sorry
+  : (runit (φ := φ) (ty := ty) (Γ := Γ) (L := L)).Pure := ⟨_, runit_eq_ret⟩
 
-theorem Eqv.Pure.runit_inv {ty : Ty α} {Γ : Ctx α ε} {L : LCtx α}
-  : (runit_inv (φ := φ) (ty := ty) (Γ := Γ) (L := L)).Pure := sorry
-
-theorem Eqv.runit_runit_inv_helper {ty : Ty α} {Γ : Ctx α ε} {L : LCtx α}
-  : runit (φ := φ) (ty := ty) (Γ := Γ) (L := L) ;; runit_inv
+theorem Eqv.pi_l_runit_helper {Γ : Ctx α ε} {L : LCtx α}
+  : pi_l (φ := φ) (A := A) (B := Ty.unit) (Γ := Γ) (L := L) ;; runit
   = let2 (var 0 ⟨by simp, le_refl _⟩)
     (let1 (unit ⊥) (ret $ pair (var 2 (by simp)) (var 0 (by simp)))) := by
   rw [let1_beta]
   rfl
 
-theorem Eqv.runit_runit_inv {ty : Ty α} {Γ : Ctx α ε} {L : LCtx α}
-  : runit (φ := φ) (ty := ty) (Γ := Γ) (L := L) ;; runit_inv = nil := by
-  rw [runit_runit_inv_helper, terminal _ (var 0 (by simp)), let1_beta]
+theorem Eqv.pi_l_runit {Γ : Ctx α ε} {L : LCtx α}
+  : pi_l (φ := φ) (A := A) (B := Ty.unit) (Γ := Γ) (L := L) ;; runit = nil := by
+  rw [pi_l_runit_helper, terminal _ (var 0 (by simp)), let1_beta]
   apply repack
 
-theorem Eqv.runit_inv_runit {ty : Ty α} {Γ : Ctx α ε} {L : LCtx α}
-  : runit_inv (φ := φ) (ty := ty) (Γ := Γ) (L := L) ;; runit = nil := by
-  stop
-  simp only [runit_inv, runit, ret_seq]
-  rw [vwk1, vwk_let2, vsubst_let2, wk_var, subst_var]
-  simp only [Nat.liftWk_zero, Term.Subst.InS.get_0_subst0, Set.mem_setOf_eq]
-  rw [let2_pair, let1_beta, let1_beta]
-  rfl
+theorem Eqv.runit_pi_l {ty : Ty α} {Γ : Ctx α ε} {L : LCtx α}
+  : runit (φ := φ) (ty := ty) (Γ := Γ) (L := L) ;; pi_l = nil := by
+  simp only [runit_eq_ret, pi_l_eq_ret, ret_ret, Term.Eqv.runit_pi_l, ret_nil]
 
-theorem Eqv.ltimes_runit {ty : Ty α} {Γ : Ctx α ε} {L : LCtx α}
-  (r : Eqv φ (⟨A, ⊥⟩::Γ) (B::L))
-  : r ⋉ Ty.unit ;; runit = runit ;; r := sorry
-
-def Eqv.lunit {ty : Ty α} {Γ : Ctx α ε} {L : LCtx α}
-  : Eqv φ (⟨Ty.unit.prod ty, ⊥⟩::Γ) (ty::L)
+def Eqv.pi_r {A B : Ty α} {Γ : Ctx α ε} {L : LCtx α}
+  : Eqv φ (⟨A.prod B, ⊥⟩::Γ) (B::L)
   := let2 (var 0 Ctx.Var.shead) (ret $ var 0 (by simp))
 
-def Eqv.lunit_inv {ty : Ty α} {Γ : Ctx α ε} {L : LCtx α}
+def Eqv.lunit {ty : Ty α} {Γ : Ctx α ε} {L : LCtx α}
   : Eqv φ (⟨ty, ⊥⟩::Γ) (Ty.unit.prod ty::L)
   := ret $ (pair (unit _) (var 0 Ctx.Var.shead))
 
+theorem Eqv.pi_r_eq_ret {Γ : Ctx α ε} {L : LCtx α}
+  : Eqv.pi_r (φ := φ) (A := A) (B := B) (Γ := Γ) (L := L) = Eqv.ret Term.Eqv.pi_r := by
+  simp only [Eqv.pi_r, let2_ret]
+  rfl
+
+theorem Eqv.lunit_eq_ret {ty : Ty α} {Γ : Ctx α ε} {L : LCtx α}
+  : Eqv.lunit (φ := φ) (ty := ty) (Γ := Γ) (L := L) = Eqv.ret Term.Eqv.lunit := by
+  simp only [Eqv.lunit, ret_ret]
+  rfl
+
+theorem Eqv.Pure.pi_r {Γ : Ctx α ε} {L : LCtx α}
+  : (pi_r (φ := φ) (A := A) (B := B) (Γ := Γ) (L := L)).Pure := ⟨_, pi_r_eq_ret⟩
+
 theorem Eqv.Pure.lunit {ty : Ty α} {Γ : Ctx α ε} {L : LCtx α}
-  : (lunit (φ := φ) (ty := ty) (Γ := Γ) (L := L)).Pure := sorry
+  : (lunit (φ := φ) (ty := ty) (Γ := Γ) (L := L)).Pure := ⟨_, lunit_eq_ret⟩
 
-theorem Eqv.Pure.lunit_inv {ty : Ty α} {Γ : Ctx α ε} {L : LCtx α}
-  : (lunit_inv (φ := φ) (ty := ty) (Γ := Γ) (L := L)).Pure := sorry
+theorem Eqv.pi_r_lunit {Γ : Ctx α ε} {L : LCtx α}
+  : pi_r (φ := φ) (A := Ty.unit) (B := B) (Γ := Γ) (L := L) ;; lunit = nil
+  := by simp only [pi_r_eq_ret, lunit_eq_ret, ret_ret, Term.Eqv.pi_r_lunit, ret_nil]
 
-theorem Eqv.lunit_seq_lunit_inv {ty : Ty α} {Γ : Ctx α ε} {L : LCtx α}
-  : lunit (φ := φ) (ty := ty) (Γ := Γ) (L := L) ;; lunit_inv = nil
-  := sorry
+theorem Eqv.lunit_pi_r {ty : Ty α} {Γ : Ctx α ε} {L : LCtx α}
+  : lunit (φ := φ) (ty := ty) (Γ := Γ) (L := L) ;; pi_r = nil
+  := by simp only [pi_r_eq_ret, lunit_eq_ret, ret_ret, Term.Eqv.lunit_pi_r, ret_nil]
 
-theorem Eqv.lunit_inv_lunit {ty : Ty α} {Γ : Ctx α ε} {L : LCtx α}
-  : lunit_inv (φ := φ) (ty := ty) (Γ := Γ) (L := L) ;; lunit = nil
-  := sorry
+theorem Eqv.lunit_braid {Γ : Ctx α ε} {L : LCtx α}
+  : (lunit (φ := φ) (ty := ty) (Γ := Γ) (L := L)) ;; braid = runit := by sorry
 
--- TODO: braid ;; lunit = runit, lunit_inv ;; braid = runit_inv, and vice versa...
+theorem Eqv.runit_braid {Γ : Ctx α ε} {L : LCtx α}
+  : (runit (φ := φ) (ty := ty) (Γ := Γ) (L := L)) ;; braid = lunit := by sorry
 
-theorem Eqv.rtimes_lunit {ty : Ty α} {Γ : Ctx α ε} {L : LCtx α}
+theorem Eqv.braid_pi_l {Γ : Ctx α ε} {L : LCtx α}
+  : braid ;; pi_l (φ := φ) (A := A) (B := B) (Γ := Γ) (L := L) = pi_r := by sorry
+
+theorem Eqv.braid_pi_r {Γ : Ctx α ε} {L : LCtx α}
+  : braid ;; pi_r (φ := φ) (A := A) (B := B) (Γ := Γ) (L := L) = pi_l
+  := by rw [<-braid_pi_l, <-seq_assoc, braid_braid, nil_seq]
+
+theorem Eqv.rtimes_pi_r {Γ : Ctx α ε} {L : LCtx α}
   (r : Eqv φ (⟨A, ⊥⟩::Γ) (B::L))
-  : Ty.unit ⋊ r ;; lunit = lunit ;; r
+  : Ty.unit ⋊ r ;; pi_r = pi_r ;; r
   := sorry
+
+theorem Eqv.ltimes_pi_l {Γ : Ctx α ε} {L : LCtx α}
+  (r : Eqv φ (⟨A, ⊥⟩::Γ) (B::L)) : r ⋉ Ty.unit ;; pi_l = pi_l ;; r := by
+  rw [<-braid_rtimes_braid, seq_assoc, braid_pi_l, seq_assoc, rtimes_pi_r, <-seq_assoc, braid_pi_r]
 
 theorem Eqv.Pure.central_left {A A' B B' : Ty α} {Γ : Ctx α ε} {L : LCtx α}
   {l : Eqv φ (⟨A, ⊥⟩::Γ) (A'::L)}
   (hl : l.Pure)
   (r : Eqv φ (⟨B, ⊥⟩::Γ) (B'::L))
-  : (l ⋉ B) ;; (A' ⋊ r) = (A ⋊ r) ;; (l ⋉ B') := sorry
+  : (l ⋉ B) ;; (A' ⋊ r) = (A ⋊ r) ;; (l ⋉ B') := by
+  let ⟨p, hp⟩ := hl;
+  simp only [hp, ltimes_eq_ret, ret_seq, Eqv.rtimes]
+  sorry
 
 theorem Eqv.Pure.central_right {A A' B B' : Ty α} {Γ : Ctx α ε} {L : LCtx α}
   (l : Eqv φ (⟨A, ⊥⟩::Γ) (A'::L))
@@ -210,19 +262,28 @@ def Eqv.assoc_inv {A B C : Ty α} {Γ : Ctx α ε} {L : LCtx α}
   let2 (var 0 ⟨by simp, le_refl _⟩) $
   ret $ pair (pair (var 3 (by simp)) (var 1 (by simp))) (var 0 (by simp))
 
+theorem Eqv.assoc_eq_ret {A B C : Ty α} {Γ : Ctx α ε} {L : LCtx α}
+  : Eqv.assoc (φ := φ) (A := A) (B := B) (C := C) (Γ := Γ) (L := L) = Eqv.ret Term.Eqv.assoc := by
+  simp only [Eqv.assoc, let2_ret]
+  rfl
+
 theorem Eqv.Pure.assoc {A B C : Ty α} {Γ : Ctx α ε} {L : LCtx α}
-  : (assoc (φ := φ) (A := A) (B := B) (C := C) (Γ := Γ) (L := L)).Pure := sorry
+  : (assoc (φ := φ) (A := A) (B := B) (C := C) (Γ := Γ) (L := L)).Pure := ⟨_, assoc_eq_ret⟩
+
+theorem Eqv.assoc_inv_eq_ret {A B C : Ty α} {Γ : Ctx α ε} {L : LCtx α}
+  : Eqv.assoc_inv (φ := φ) (A := A) (B := B) (C := C) (Γ := Γ) (L := L) = Eqv.ret Term.Eqv.assoc_inv
+  := by simp only [Eqv.assoc_inv, let2_ret]; rfl
 
 theorem Eqv.Pure.assoc_inv {A B C : Ty α} {Γ : Ctx α ε} {L : LCtx α}
-  : (assoc_inv (φ := φ) (A := A) (B := B) (C := C) (Γ := Γ) (L := L)).Pure := sorry
+  : (assoc_inv (φ := φ) (A := A) (B := B) (C := C) (Γ := Γ) (L := L)).Pure := ⟨_, assoc_inv_eq_ret⟩
 
 theorem Eqv.assoc_assoc_inv {A B C : Ty α} {Γ : Ctx α ε} {L : LCtx α}
   : assoc (φ := φ) (A := A) (B := B) (C := C) (Γ := Γ) (L := L) ;; assoc_inv = nil
-  := sorry
+  := by simp only [assoc_eq_ret, assoc_inv_eq_ret, ret_ret, Term.Eqv.assoc_assoc_inv, ret_nil]
 
 theorem Eqv.assoc_inv_assoc {A B C : Ty α} {Γ : Ctx α ε} {L : LCtx α}
   : assoc_inv (φ := φ) (A := A) (B := B) (C := C) (Γ := Γ) (L := L) ;; assoc = nil
-  := sorry
+  := by simp only [assoc_eq_ret, assoc_inv_eq_ret, ret_ret, Term.Eqv.assoc_inv_assoc, ret_nil]
 
 theorem Eqv.assoc_left_nat {A B C A' : Ty α} {Γ : Ctx α ε} {L : LCtx α}
   (l : Eqv φ (⟨A, ⊥⟩::Γ) (A'::L))
@@ -237,8 +298,8 @@ theorem Eqv.assoc_right_nat {A B C C' : Ty α} {Γ : Ctx α ε} {L : LCtx α}
   : (A.prod B) ⋊ r ;; assoc = assoc ;; A ⋊ (B ⋊ r) := sorry
 
 theorem Eqv.triangle {X Y : Ty α} {Γ : Ctx α ε} {L : LCtx α}
-  : assoc (φ := φ) (Γ := Γ) (L := L) (A := X) (B := Ty.unit) (C := Y) ;; X ⋊ lunit
-  = runit ⋉ Y := sorry
+  : assoc (φ := φ) (Γ := Γ) (L := L) (A := X) (B := Ty.unit) (C := Y) ;; X ⋊ pi_r
+  = pi_l ⋉ Y := sorry
 
 theorem Eqv.pentagon {W X Y Z : Ty α} {Γ : Ctx α ε} {L : LCtx α}
   : assoc (φ := φ) (Γ := Γ) (L := L) (A := W.prod X) (B := Y) (C := Z) ;; assoc
